Valaig/Aig/Lemmas.lean
@@ -1,54 +1,105 @@
 import Valaig.Aig.Basic
 
-namespace Valaig.Aig
+namespace Valaig
 
-variable {aig : Aig} {var : Var}
+attribute [local grind] Aig.Raw.aig
+attribute [local grind! .] Std.Sat.AIG.hzero
+attribute [local grind! .] Std.Sat.AIG.hconst
+attribute [local grind! .] Aig.hfalse
+attribute [local grind! .] Aig.hinputs
+attribute [local grind! .] Aig.hlatches
 
-theorem nextInputIdx_notIn_decls (aig : Aig) {i : Nat} (h : i < aig.size) :
-    aig.aig.decls[i] ≠ .atom (.input aig.nextInputIdx) := by
-  intro heq
-  have := aig.hinputs.hsurjec h (iarr := aig.nextInputIdx) heq
+section
+variable {aig : Aig.Raw}
+
+theorem Var.validIn_def {var : Var} :
+    var.validIn aig ↔ var.idx < aig.size := by
+  simp_all only [Aig.Raw.size, Var.validIn]
+
+@[simp, grind! .]
+theorem Var.constant_validIn : Var.constant.validIn aig := by
+  simp [Var.validIn, Var.constant, aig.aig.hzero, Aig.Raw.size]
+
+@[simp, grind! .]
+theorem Lit.validIn_mk_validIn {var : Var} (h : var.validIn aig) {invert : Bool} :
+    Lit.mk var invert |>.validIn aig := by
+  simp_all only [Var.validIn, Aig.Raw.size, Lit.mk_var]
+
+end
+
+namespace Aig
+
+theorem getElem_def {v : Var} (h : v.validIn aig) :
+    aig[v] = aig.aig.decls[v.idx] := by
+  simp_all only [Raw.instGetElemVar]
+
+attribute [local simp, local grind =] getElem_def
+attribute [local simp, local grind] Raw.size
+attribute [local simp, local grind .] Array.getElem_of_mem
+
+variable {aig : Aig}
+
+@[simp, grind =]
+theorem mem_iff_getElem {a : Std.Sat.AIG.Decl AtomIdx}  :
+    a ∈ aig ↔ ∃ (v : Var), ∃ (h : v.validIn aig), aig[v] = a := by
+  simp only [instMem, Raw.instMem, Array.mem_iff_getElem]
+  constructor
+  · rintro ⟨i, h⟩
+    exists Var.ofIdx i
+  · rintro ⟨v, h⟩
+    exists v.idx
+
+theorem nextInputIdx_not_mem_aig :
+    .atom (.input aig.nextInputIdx) ∉ aig:= by
+  simp
+  intro _ h
+  have := aig.hinputs.hsurjec h (iarr := aig.nextInputIdx)
   grind only [nextInputIdx]
 
-theorem nextLatchIdx_notIn_decls (aig : Aig) {i : Nat} (h : i < aig.size) :
-    aig.aig.decls[i] ≠ .atom (.latch aig.nextLatchIdx) := by
-  intro heq
-  have := aig.hlatches.hsurjec h (iarr := aig.nextLatchIdx) heq
+theorem nextLatchIdx_not_mem_aig :
+    .atom (.latch aig.nextLatchIdx) ∉ aig:= by
+  simp
+  intro _ h
+  have := aig.hlatches.hsurjec h (iarr := aig.nextLatchIdx)
   grind only [nextLatchIdx]
 
+theorem decls_unique_inputs {i j : Nat}
+    (hi : i < aig.size)
+    (hj : j < aig.size)
+    (hatom : aig.aig.decls[i] matches .atom (.input _))
+    (heq : aig.aig.decls[i] = aig.aig.decls[j]) :
+    i = j := by
+  have {iarr : Nat} := aig.hinputs.hsurjec hi (iarr := iarr)
+  have {iarr : Nat} := aig.hinputs.hsurjec hj (iarr := iarr)
+  grind only
 
-theorem decls_unique_inputs :
-    ∀ {i j} (hi : i < aig.size) (hj : j < aig.size),
-      aig.aig.decls[i] matches .atom (.input _) ∧ aig.aig.decls[i] = aig.aig.decls[j] →
-      i = j := by
-  grind
+theorem decls_unique_latches {i j : Nat}
+    (hi : i < aig.size)
+    (hj : j < aig.size)
+    (hatom : aig.aig.decls[i] matches .atom (.latch _))
+    (heq : aig.aig.decls[i] = aig.aig.decls[j]) :
+    i = j := by
+  have {iarr : Nat} := aig.hlatches.hsurjec hi (iarr := iarr)
+  have {iarr : Nat} := aig.hlatches.hsurjec hj (iarr := iarr)
+  grind only
 
-theorem decls_unique_latches :
-    ∀ {i j} (hi : i < aig.size) (hj : j < aig.size),
-      aig.aig.decls[i] matches .atom (.latch _) ∧ aig.aig.decls[i] = aig.aig.decls[j] →
-      i = j := by
-  grind
+theorem decls_unique_atoms {i j : Nat}
+    (hi : i < aig.size)
+    (hj : j < aig.size)
+    (hatom : aig.aig.decls[i] matches .atom _)
+    (heq : aig.aig.decls[i] = aig.aig.decls[j]) :
+    i = j := by
+  match h : aig.aig.decls[i], hatom with
+  | .atom (.input _), _ => grind only [decls_unique_inputs]
+  | .atom (.latch _), _ => grind only [decls_unique_latches]
 
-theorem decls_unique_atoms :
-    ∀ {i j} (hi : i < aig.size) (hj : j < aig.size),
-      aig.aig.decls[i] matches .atom _ ∧ aig.aig.decls[i] = aig.aig.decls[j] →
-      i = j := by
-  intro i j hi hj
-  match h : aig.aig.decls[i] with
-  | .false => simp
-  | .gate _ _ => simp
-  | .atom (.input _) => grind only [decls_unique_inputs]
-  | .atom (.latch _) => grind only [decls_unique_latches]
+theorem inputs_unique {i j : Nat} (hi : i < aig.numInputs) (hj : j < aig.numInputs)
+    (heq : aig.inputs[i].var = aig.inputs[j].var) : i = j := by
+  grind only [hinputs]
 
-theorem inputs_unique :
-    ∀ {i j} (hi : i < aig.numInputs) (hj : j < aig.numInputs),
-      aig.inputs[i].var = aig.inputs[j].var → i = j := by
-  grind
-
-theorem latches_unique :
-    ∀ {i j} (hi : i < aig.numLatches) (hj : j < aig.numLatches),
-      aig.latches[i].var = aig.latches[j].var → i = j := by
-  grind
+theorem latches_unique {i j : Nat} (hi : i < aig.numLatches) (hj : j < aig.numLatches)
+    (heq : aig.latches[i].var = aig.latches[j].var) : i = j := by
+  grind only [hlatches]
 
 @[simp, grind! .]
 theorem empty_inputs :
@@ -60,26 +111,38 @@ theorem empty_latches :
     empty.latches = #[] := by
   simp only [empty]
 
+@[simp, grind! .]
+theorem input_mem_validIn {input : Input} (hmem : input ∈ aig.inputs) :
+    input.var.validIn aig := by
+  grind only [Array.getElem_of_mem, hinputs, =Var.validIn_def, Raw.size]
+
+@[simp, grind! .]
+theorem latch_mem_validIn {latch : Latch} (hmem : latch ∈ aig.latches) :
+    latch.var.validIn aig := by
+  grind only [Array.getElem_of_mem, hlatches, =Var.validIn_def, Raw.size]
+
+@[simp, grind! .]
+theorem input_mem_matches_input {input : Input} (hmem : input ∈ aig.inputs) :
+    aig[input.var]'(input_mem_validIn hmem) matches .atom (.input _) := by
+  grind only [hinputs, Array.getElem_of_mem, getElem_def]
+
+@[simp, grind! .]
+theorem latch_mem_matches_latch {latch : Latch} (hmem : latch ∈ aig.latches) :
+    aig[latch.var]'(latch_mem_validIn hmem) matches .atom (.latch _) := by
+  grind only [!hlatches, Array.getElem_of_mem, getElem_def]
+
 section
+variable {aig : Aig} {var : Var}
+variable {symbol : String}
+variable {rhs0 rhs1 : Lit} {h0 : rhs0.validIn aig} {h1 : rhs1.validIn aig}
+variable {next : Lit} {reset : Option Lit}
 
 attribute [local simp] mkAtom_eq_decls_push
 attribute [local simp] mkAtom_ref_eq_decls_size
 attribute [local simp] Std.Sat.AIG.mkAtom_le_size
 attribute [local simp] Std.Sat.AIG.mkAndCached_le_size
 
-variable {symbol : String}
-variable {rhs0 rhs1 : Lit} {h0 : rhs0.validIn aig} {h1 : rhs1.validIn aig}
-variable {next : Lit} {reset : Option Lit}
-
-@[grind! .]
-theorem Var.constant_validIn : Var.constant.validIn aig := by
-  simp [Var.validIn, Var.constant, aig.aig.hzero]
-
-@[grind! .]
-theorem Lit.validIn_mk_validIn (h : var.validIn aig) {invert : Bool} :
-    Lit.mk var invert |>.validIn aig := by
-  simp_all [Var.validIn]
-
+-- addInput Lemmas
 
 theorem addInput_size_ge :
     (aig.addInput symbol).fst.size ≥ aig.size := by
@@ -88,23 +151,60 @@ theorem addInput_size_ge :
 @[grind! .]
 theorem validIn_addInput (h : var.validIn aig) :
     var.validIn (aig.addInput symbol).fst := by
-  grind [addInput_size_ge, Var.validIn]
+  grind only [addInput_size_ge, Var.validIn_def]
 
 @[grind! .]
 theorem addInput_validIn :
     (aig.addInput symbol).snd.var.validIn (aig.addInput symbol).fst := by
-  simp [addInput, Var.validIn]
+  simp [addInput, Var.validIn_def]
 
+@[simp]
 theorem addInput_inputs_eq_push :
     let (aig', input) := aig.addInput symbol
     aig'.inputs = aig.inputs.push input := by
   simp [addInput]
 
 @[grind! .]
+theorem addInput_mem_inputs :
+    let (aig', input) := aig.addInput symbol
+    input ∈ aig'.inputs := by
+  grind only [addInput_inputs_eq_push, Array.mem_push]
+
+@[grind! .]
+theorem addInput_matches_atom_input :
+    let (eq:=_) (aig', input) := aig.addInput symbol
+    aig'[input.var]'(by grind only [addInput_validIn]) matches .atom (.input _) := by
+  apply input_mem_matches_input
+  exact addInput_mem_inputs
+
+@[grind! .]
+theorem addInput_matches_atom :
+    let (eq:=_) (aig', input) := aig.addInput symbol
+    aig'[input.var]'(by grind only [addInput_validIn]) matches .atom _ := by
+  grind only [addInput_matches_atom_input]
+
+@[simp, grind! .]
 theorem addInput_latches_eq :
     (aig.addInput symbol).fst.latches = aig.latches := by
   simp [addInput]
 
+@[simp, grind! .]
+theorem addInput_getElem_eq {var : Var} (h : var.validIn aig) :
+    (aig.addInput symbol).fst[var]'(validIn_addInput h) = aig[var] := by
+  rw [Var.validIn_def] at h
+  simp_all [addInput, Array.getElem_push_lt]
+
+@[grind! .]
+theorem addInput_mem_eq {decl} (h : decl ∈ aig) :
+    decl ∈ (aig.addInput symbol).fst := by
+  rw [mem_iff_getElem] at *
+  rcases h with ⟨v, ⟨h, heq⟩⟩
+  exists v
+  exists (validIn_addInput h)
+  rw [←heq]
+  apply addInput_getElem_eq
+
+-- addLatch Lemmas
 
 theorem addLatch_size_ge :
     (aig.addLatch next reset symbol).fst.size ≥ aig.size := by
@@ -113,23 +213,60 @@ theorem addLatch_size_ge :
 @[grind! .]
 theorem validIn_addLatch (h : var.validIn aig) :
     var.validIn (aig.addLatch next reset symbol).fst := by
-  grind [addLatch_size_ge, Var.validIn]
+  grind only [addLatch_size_ge, Var.validIn_def]
 
 @[grind! .]
 theorem addLatch_validIn:
     (aig.addLatch next reset symbol).snd.var.validIn (aig.addLatch next reset symbol).fst := by
-  simp [addLatch, Var.validIn]
+  simp [addLatch, Var.validIn_def]
 
+@[simp]
 theorem addLatch_latches_eq_push :
     let (aig', latch) := aig.addLatch next reset symbol
     aig'.latches = aig.latches.push latch := by
   simp [addLatch]
 
 @[grind! .]
+theorem addLatch_mem_latches :
+    let (aig', latch) := aig.addLatch next reset symbol
+    latch ∈ aig'.latches := by
+  grind only [addLatch_latches_eq_push, Array.mem_push]
+
+@[grind! .]
+theorem addLatch_matches_atom_latch :
+    let (eq:=_) (aig', latch) := aig.addLatch next reset symbol
+    aig'[latch.var]'(by grind only [addLatch_validIn]) matches .atom (.latch _) := by
+  apply latch_mem_matches_latch
+  exact addLatch_mem_latches
+
+@[grind! .]
+theorem addLatch_matches_atom :
+    let (eq:=_) (aig', latch) := aig.addLatch next reset symbol
+    aig'[latch.var]'(by grind only [addLatch_validIn]) matches .atom _ := by
+  grind only [addLatch_matches_atom_latch]
+
+@[simp, grind! .]
 theorem addLatch_inputs_eq :
     (aig.addLatch next reset symbol).fst.inputs = aig.inputs := by
   simp [addLatch]
 
+@[simp, grind! .]
+theorem addLatch_getElem_eq {var : Var} (h : var.validIn aig) :
+    (aig.addLatch next reset symbol).fst[var]'(validIn_addLatch h) = aig[var] := by
+  rw [Var.validIn_def] at h
+  simp_all [addLatch, Array.getElem_push_lt]
+
+@[grind! .]
+theorem addLatch_mem_eq {decl} (h : decl ∈ aig) :
+    decl ∈ (aig.addLatch next reset symbol).fst := by
+  rw [mem_iff_getElem] at *
+  rcases h with ⟨v, ⟨h, heq⟩⟩
+  exists v
+  exists (validIn_addLatch h)
+  rw [←heq]
+  apply addLatch_getElem_eq
+
+-- addLatch' Lemmas
 
 theorem addLatch'_size_ge :
     (aig.addLatch' reset symbol).fst.size ≥ aig.size := by
@@ -138,23 +275,60 @@ theorem addLatch'_size_ge :
 @[grind! .]
 theorem validIn_addLatch' (h : var.validIn aig) :
     var.validIn (aig.addLatch' reset symbol).fst := by
-  grind [addLatch'_size_ge, Var.validIn]
+  grind only [addLatch'_size_ge, Var.validIn_def]
 
 @[grind! .]
 theorem addLatch'_validIn:
     (aig.addLatch' reset symbol).snd.var.validIn (aig.addLatch' reset symbol).fst := by
-  simp [addLatch', Var.validIn]
+  simp [addLatch', Var.validIn_def]
 
+@[simp]
 theorem addLatch'_latches_eq_push :
     let (aig', latch) := aig.addLatch' reset symbol
     aig'.latches = aig.latches.push latch := by
   simp [addLatch']
 
 @[grind! .]
+theorem addLatch'_mem_latches :
+    let (aig', latch) := aig.addLatch' reset symbol
+    latch ∈ aig'.latches := by
+  grind only [addLatch'_latches_eq_push, Array.mem_push]
+
+@[grind! .]
+theorem addLatch'_matches_atom_latch :
+    let (eq:=_) (aig', latch) := aig.addLatch' reset symbol
+    aig'[latch.var]'(by grind only [addLatch'_validIn]) matches .atom (.latch _) := by
+  apply latch_mem_matches_latch
+  exact addLatch'_mem_latches
+
+@[grind! .]
+theorem addLatch'_matches_atom :
+    let (eq:=_) (aig', latch) := aig.addLatch' reset symbol
+    aig'[latch.var]'(by grind only [addLatch'_validIn]) matches .atom _ := by
+  grind only [addLatch'_matches_atom_latch]
+
+@[simp, grind! .]
 theorem addLatch'_inputs_eq :
     (aig.addLatch' reset symbol).fst.inputs = aig.inputs := by
   simp [addLatch']
 
+@[simp, grind! .]
+theorem addLatch'_getElem_eq {var : Var} (h : var.validIn aig) :
+    (aig.addLatch' reset symbol).fst[var]'(validIn_addLatch' h) = aig[var] := by
+  rw [Var.validIn_def] at h
+  simp_all [addLatch', Array.getElem_push_lt]
+
+@[grind! .]
+theorem addLatch'_mem_eq {decl} (h : decl ∈ aig) :
+    decl ∈ (aig.addLatch' reset symbol).fst := by
+  rw [mem_iff_getElem] at *
+  rcases h with ⟨v, ⟨h, heq⟩⟩
+  exists v
+  exists (validIn_addLatch' h)
+  rw [←heq]
+  apply addLatch'_getElem_eq
+
+-- addGate Lemmas
 
 theorem addGate_size_ge :
     (aig.addGate rhs0 rhs1 h0 h1).fst.size ≥ aig.size := by
@@ -163,31 +337,79 @@ theorem addGate_size_ge :
 @[grind! .]
 theorem validIn_addGate (h : var.validIn aig) :
     var.validIn (aig.addGate rhs0 rhs1 h0 h1).fst := by
-  grind [addGate_size_ge, Var.validIn]
+  grind only [addGate_size_ge, Var.validIn_def]
 
 @[grind! .]
 theorem addGate_validIn:
     (aig.addGate rhs0 rhs1 h0 h1).snd.validIn (aig.addGate rhs0 rhs1 h0 h1).fst := by
-  simp [addGate, Var.validIn]
-  have (r : Std.Sat.AIG.Entrypoint Aig.Atom) := r.ref.hgate
-  grind
+  simp [addGate, Var.validIn_def]
+  have (r : Std.Sat.AIG.Entrypoint Aig.AtomIdx) := r.ref.hgate
+  grind only
 
-@[grind! .]
+@[simp, grind! .]
 theorem addGate_inputs_eq :
     (aig.addGate rhs0 rhs1 h0 h1).fst.inputs = aig.inputs := by
   simp [addGate]
 
-@[grind! .]
+@[simp, grind! .]
 theorem addGate_latches_eq :
     (aig.addGate rhs0 rhs1 h0 h1).fst.latches = aig.latches := by
   simp [addGate]
+
+@[simp, grind! .]
+theorem addGate_getElem_eq {var : Var} (h : var.validIn aig) :
+    (aig.addGate rhs0 rhs1 h0 h1).fst[var]'(validIn_addGate h) = aig[var] := by
+  apply Std.Sat.AIG.mkGateCached_decl_eq
+
+@[grind! .]
+theorem addGate_mem_eq {decl} (h : decl ∈ aig) :
+    decl ∈ (aig.addGate rhs0 rhs1 h0 h1).fst := by
+  rw [mem_iff_getElem] at *
+  rcases h with ⟨v, ⟨h, heq⟩⟩
+  exists v
+  exists (validIn_addGate h)
+  rw [←heq]
+  apply addGate_getElem_eq
 
 end
 
 section
 
+-- TODO: These proofs are messy
+
 variable {nextState : (latch : Latch) -> latch ∈ aig.latches -> Lit.In aig}
-variable {state : FinaliseLatchesState aig}
+variable {init state : finaliseLatches.State aig}
+
+structure finaliseLatches.induction (nextState : (latch : Latch) -> latch ∈ aig.latches -> Lit.In aig) where
+  motive (init state : State aig) : Prop
+  hinit : motive (.empty aig) (.empty aig)
+  htrans (init state : State aig) (hidx : state.idx ≥ init.idx) {h} :
+    motive init state -> motive init (step aig nextState state h)
+
+theorem finaliseLatches.induction.lift' (thm : induction nextState)
+    (hmotive : thm.motive init state) (hidx : state.idx ≥ init.idx) :
+    thm.motive init (updateLatches aig nextState (s := state)) := by
+  induction h : (state.latches.size - state.idx) generalizing state with
+  | zero =>
+    unfold updateLatches
+    grind only
+  | succ n' ih =>
+    unfold updateLatches
+    split
+    · trivial
+    · simp_all
+      apply ih
+      · apply thm.htrans
+        · exact hidx
+        · exact hmotive
+      · grind only [State.hsize]
+      · grind only [State.hsize]
+
+theorem finaliseLatches.induction.lift (thm : induction nextState) :
+    thm.motive (.empty aig) (updateLatches aig nextState (s := .empty aig)) := by
+  apply lift'
+  · exact thm.hinit
+  · omega
 
 theorem finaliseLatches.updateLatches_size_const :
     let state' := (finaliseLatches.updateLatches aig nextState (s := state))
@@ -195,42 +417,87 @@ theorem finaliseLatches.updateLatches_size_const :
   intro state'
   simp_all only [state.hsize, state'.hsize]
 
-theorem finaliseLatches.updateLatches_modified_once :
+def finaliseLatches.modified_once : induction nextState := {
+  motive init state := ∀ {i} (_ : i < state.latches.size) (_ : i < init.idx),
+    state.latches[i] = init.latches[i]'(by grind only [updateLatches_size_const])
+
+  hinit := by grind only
+  htrans := by
+    intro init state _ _ _ i
+    unfold step
+    by_cases h : state.latches[state.idx].next.isSome
+    · rcases Option.isSome_iff_exists.mp h with ⟨latch, heq⟩
+      grind only
+    · grind only [Array.getElem_modify]
+}
+
+def finaliseLatches.next_eq_some : induction nextState := {
+  motive init state := 
+    ∀ {i} (_ : i < state.latches.size) (_ : i < state.idx),
+      state.latches[i].next.isSome
+
+  hinit := by grind only [State.empty],
+
+  htrans := by
+    intro init state hidx h ha i hi _
+    unfold step
+    by_cases h : state.latches[state.idx].next.isSome
+    · rcases Option.isSome_iff_exists.mp h with ⟨latch, heq⟩
+      grind only
+    · simp_all
+      by_cases i = state.idx
+      · simp_all [Array.getElem_modify_self]
+      · rw [Array.getElem_modify_of_ne]
+        · apply ha
+          grind only
+        · cutsat
+}
+
+theorem finaliseLatches.updateLatches_idx_eq_size_ind (h : state.idx ≤ state.latches.size) :
     let state' := (finaliseLatches.updateLatches aig nextState (s := state))
-    ∀ {i} (_ : i < state'.latches.size) (_ : i < state.idx),
-      state'.latches[i] = state.latches[i]'(by grind [updateLatches_size_const]) := by
+    state'.idx = state'.latches.size := by
   induction h : (state.latches.size - state.idx) generalizing state with
-  | zero => grind only [updateLatches]
+  | zero =>
+    unfold updateLatches
+    grind only
   | succ n' ih =>
-    dsimp only
-    intro i h1 h2
-    by_cases i ≠ state.idx
-    · by_cases state.latches[state.idx].next.isSome
-      · grind only [updateLatches, hlatches, updateLatches_size_const, Option.isSome_none]
-      · grind only [updateLatches, Array.size_modify, hlatches, Array.getElem_modify]
-    · grind only [updateLatches]
+    unfold updateLatches
+    simp_all
+    split
+    · cutsat
+    · apply ih
+      · simp [State.hsize] at *
+        grind
+      · grind only [State.hsize]
+
+theorem finaliseLatches.updateLatches_idx_eq_size :
+    let state' := (finaliseLatches.updateLatches aig nextState)
+    state'.idx = state'.latches.size := by
+  apply updateLatches_idx_eq_size_ind
+  · simp only [State.empty, Nat.zero_le]
 
 theorem finaliseLatches.updateLatches_next_eq_some :
-    let state' := (finaliseLatches.updateLatches aig nextState (s := state))
-    ∀ {i} (_ : i < state'.latches.size) (_ : i ≥ state.idx),
-      state'.latches[i].next.isSome := by
-  induction h : (state.latches.size - state.idx) generalizing state with
-  | zero => grind only [updateLatches]
-  | succ n' ih =>
-    grind only [updateLatches, hlatches, updateLatches_modified_once, Option.isSome_some, Array.getElem_modify]
+    let state' := (finaliseLatches.updateLatches aig nextState)
+    ∀ {i} (_ : i < state'.latches.size), state'.latches[i].next.isSome := by
+  intros
+  apply next_eq_some.lift
+  · grind only [updateLatches_idx_eq_size]
 
 theorem finaliseLatches_WF :
     aig.finaliseLatches nextState |>.WF := by
   constructor
-  · simp only [finaliseLatches]
-    grind [Array.mem_def, List.mem_iff_getElem, finaliseLatches.updateLatches_next_eq_some]
+  · grind only [finaliseLatches, Array.mem_iff_getElem, finaliseLatches.updateLatches_next_eq_some]
 
 theorem finaliseLatches_aig_eq :
     (aig.finaliseLatches nextState).aig = aig.aig := by
   simp only [finaliseLatches]
 
+theorem finaliseLatches_inputs_eq :
+    (aig.finaliseLatches nextState).inputs = aig.inputs := by
+  simp only [finaliseLatches]
+
 @[grind! .]
-theorem validIn_finaliseLatches (h : var.validIn aig) :
+theorem validIn_finaliseLatches {var : Var} (h : var.validIn aig) :
     var.validIn (aig.finaliseLatches nextState) := by
   simp_all only [Var.validIn, Raw.size, finaliseLatches_aig_eq]
 
