Valaig/Aig/FromStd.lean
@@ -25,29 +25,38 @@ private structure FromStdState (stdAig : AIG α) where
   aig : Aig := .empty
   -- A map from variable indices in stdAig (Ref.gate) to Vars in aig
   map : Array Var := #[]
+  -- A map from atoms in the original AIG to their canonical variable in aig
+  atomMap : Std.HashMap α Var := .emptyWithCapacity
   -- A map from the variable defined by each latch to its ref in stdAig, to
   -- allow latch finalisation once all nodes have been visited
   latchNexts : Std.HashMap Var stdAig.Ref := .emptyWithCapacity
 
   hmap : ∀ {x} (_ : x ∈ map), x.validIn aig := by grind
   hlatch : ∀ {l} (_ : l ∈ aig.latches), l.var ∈ latchNexts := by grind
+  hatom : ∀ {a} (_ : a ∈ atomMap),
+    ∃ (h : atomMap[a].validIn aig), aig[atomMap[a]] matches .atom _ := by grind
 
-def fromStdAIG (stdAig : AIG α) (relabel : α -> RelabelledAtom stdAig) : (aig : Aig) × (stdAig.Ref -> Lit.In aig) :=
+structure FromStdResult (stdAig : AIG α) where
+  aig : Aig
+  refMap : stdAig.Ref -> Lit
+  atomMap : α -> Option Var
+
+def fromStdAIG (stdAig : AIG α) (relabel : α -> RelabelledAtom stdAig) : FromStdResult stdAig :=
   have ⟨state, hstate⟩ := go
 
   let aig := state.aig.finaliseLatches fun latch h =>
     let ref := state.latchNexts[latch.var]'(state.hlatch h)
     have := ref.hgate
     let lit := state.map[ref.gate]'(by omega) |>.toLit ref.invert
-    ⟨lit, by grind⟩
+    ⟨lit, by grind only [Lit.mk_var, Array.getElem_mem]⟩
 
-  -- TODO: This duplication between this and the above is slightly annoying
-  let lookup (ref : stdAig.Ref) : Lit.In aig :=
+  let refMap (ref : stdAig.Ref) : Lit :=
     have := ref.hgate
-    let lit := state.map[ref.gate]'(by omega) |>.toLit ref.invert
-    ⟨lit, by grind⟩
+    state.map[ref.gate]'(by omega) |>.toLit ref.invert
 
-  ⟨aig, lookup⟩
+  let atomMap (atom : α) : Option Var := state.atomMap[atom]?
+
+  { aig, refMap, atomMap }
 
 where
   go (s : FromStdState stdAig := {}) : { s : FromStdState stdAig // s.map.size ≥ stdAig.decls.size } :=
@@ -56,36 +65,73 @@ where
       ⟨s, hidx⟩
     else
       match heq : stdAig.decls[idx] with
-      | .false => go { s with map := s.map.push .constant, hmap := by grind }
+      | .false =>
+        have hmap := by grind only [Array.mem_push, Var.constant_validIn]
+        go { s with map := s.map.push .constant, hmap }
       | .gate rhs0 rhs1 =>
         have hdag := stdAig.hdag (i := idx) (lhs := rhs0) (rhs := rhs1) (by omega) heq
         let rhs0 := s.map[rhs0.gate]'hdag.left |>.toLit rhs0.invert
         let rhs1 := s.map[rhs1.gate]'hdag.right |>.toLit rhs1.invert
         let (eq:=_) (aig, lhs) := s.aig.addGate rhs0 rhs1
         let map := s.map.push lhs.var
-        go { s with aig, map, hmap := by grind, hlatch := by grind }
 
-      | .atom a =>
-        match relabel a with
-        | .input symbol =>
-          let (eq :=_) (aig, lhs) := s.aig.addInput symbol
-          let map := s.map.push lhs.var
-          go { s with aig, map, hmap := by grind, hlatch := by grind }
+        have hmap := by grind only [addGate_validIn, validIn_addGate, Array.mem_push]
+        have hlatch := by grind only [addGate_latches_eq]
+        have hatom := by grind only [validIn_addGate, addGate_getElem_eq]
+        go { s with aig, map, hmap, hlatch, hatom }
 
-        | .latch next reset symbol =>
-          let (eq:=_) (aig, lhs) := s.aig.addLatch' (reset.map Lit.ofRef) symbol
-          let map := s.map.push lhs.var
-          let latchNexts := s.latchNexts.insert lhs next
-          let hlatch := by grind [addLatch'_latches_eq_push]
-          go { aig, map, latchNexts, hmap := by grind, hlatch }
+      | .atom atom =>
+        match h : s.atomMap[atom]? with
+        | some var =>
+          let map := s.map.push var
+
+          have hmap := by
+            simp_all
+            rintro _ (hold | hnew)
+            · exact s.hmap hold
+            · have := Std.HashMap.isSome_getElem?_iff_mem.mp (Option.isSome_of_eq_some h)
+              simp_all; rw [←h]; cases (s.hatom this); trivial
+          go { s with map, hmap }
+        | none =>
+          match relabel atom with
+          | .input symbol =>
+            let (eq:=_) (aig, lhs) := s.aig.addInput symbol
+            let map := s.map.push lhs.var
+            let atomMap := s.atomMap.insert atom lhs
+
+            have hmap := by grind only [addInput_validIn, validIn_addInput, Array.mem_push]
+            have hlatch := by grind only [addInput_latches_eq]
+            have hatom := by 
+              intros
+              simp only [Std.HashMap.getElem_insert]
+              split
+              · grind only [addInput_matches_atom]
+              · grind only [validIn_addInput, addInput_getElem_eq]
+            go { s with aig, map, atomMap, hmap, hlatch, hatom }
+
+          | .latch next reset symbol =>
+            let (eq:=_) (aig, lhs) := s.aig.addLatch' (reset.map Lit.ofRef) symbol
+            let map := s.map.push lhs.var
+            let atomMap := s.atomMap.insert atom lhs
+            let latchNexts := s.latchNexts.insert lhs next
+
+            have hmap := by grind only [addLatch'_validIn, validIn_addLatch', Array.mem_push]
+            have hlatch := by grind only [addLatch'_latches_eq_push, Std.HashMap.mem_insert, Array.mem_push]
+            have hatom := by 
+              intros
+              simp only [Std.HashMap.getElem_insert]
+              split
+              · grind only [addLatch'_matches_atom]
+              · grind only [validIn_addLatch', addLatch'_getElem_eq]
+            go { aig, map, atomMap, latchNexts, hmap, hlatch, hatom }
 
   termination_by stdAig.decls.size - s.map.size
 
 @[inline]
 def fromStdEntrypoint (entry : Entrypoint α) (relabel : α -> RelabelledAtom entry.aig) :
-    (aig : Aig) × Lit × (entry.aig.Ref -> Lit.In aig) :=
-  let ⟨aig, map⟩ := fromStdAIG entry.aig relabel
-  let lit := map entry.ref
-  ⟨aig, lit, map⟩
+    FromStdResult entry.aig × Lit :=
+  let result := fromStdAIG entry.aig relabel
+  let lit := result.refMap entry.ref
+  (result, lit)
 
 end Valaig.Aig
